Workaround SMT issues when implementing Steel effect combinators

ulib/experimental/Steel.Effect.fst
@@ -172,6 +172,16 @@ let req_frame frame snap =
 
 #push-options "--z3rlimit 20 --fuel 1 --ifuel 1"
 
+let frame_opaque frame h0 h1 = frame_equalities frame h0 h1
+
+unfold
+let norm_opaque = norm [delta_only [`%frame_opaque]]
+
+let lemma_frame_opaque_refl (frame:vprop) (h:rmem frame) : Lemma (frame_opaque frame h h) =
+  assert (frame_opaque frame h h) by (
+    T.norm [delta_only [`%frame_opaque]];
+    T.apply_lemma (`lemma_frame_equalities_refl))
+
 val frame00 (#a:Type)
           (#framed:bool)
           (#pre:pre_t)
@@ -186,7 +196,7 @@ val frame00 (#a:Type)
     (fun x -> post x `star` frame)
     (fun h -> req (focus_rmem h pre))
     (fun h0 r h1 -> req (focus_rmem h0 pre) /\ ens (focus_rmem h0 pre) r (focus_rmem h1 (post r)) /\
-     frame_equalities frame (focus_rmem h0 frame) (focus_rmem h1 frame))
+     frame_opaque frame (focus_rmem h0 frame) (focus_rmem h1 frame))
 
 let frame00 #a #framed #pre #post #req #ens f frame =
   fun frame' ->
@@ -210,15 +220,89 @@ let frame00 #a #framed #pre #post #req #ens f frame =
       // We proved focus_rmem h0 frame == focus_rmem h1 frame so far
 
       let h0:rmem (pre `star` frame) = mk_rmem (pre `star` frame) (core_mem m0) in
-      lemma_frame_equalities_refl frame (focus_rmem h0 frame);
+      lemma_frame_opaque_refl frame (focus_rmem h0 frame);
 
       x
 
 #pop-options
 
+let norm_repr (#a:Type) (#framed:bool)
+ (#pre:pre_t) (#post:post_t a) (#req:req_t pre) (#ens:ens_t pre a post)
+ (f:repr a framed pre post req ens) : repr a framed pre post (fun h -> norm_opaque (req h)) (fun h0 x h1 -> norm_opaque (ens h0 x h1))
+ = f
+
+unfold
+let bind_req_opaque (#a:Type)
+  (#pre_f:pre_t) (#post_f:post_t a)
+  (req_f:req_t pre_f) (ens_f:ens_t pre_f a post_f)
+  (#pre_g:a -> pre_t)
+  (#pr:a -> prop)
+  (req_g:(x:a -> req_t (pre_g x)))
+  (frame_f:vprop) (frame_g:a -> vprop)
+  (_:squash (can_be_split_forall_dep pr (fun x -> post_f x `star` frame_f) (fun x -> pre_g x `star` frame_g x)))
+: req_t (pre_f `star` frame_f)
+= fun m0 ->
+  req_f (focus_rmem m0 pre_f) /\
+  (forall (x:a) (h1:hmem (post_f x `star` frame_f)).
+    (ens_f (focus_rmem m0 pre_f) x (focus_rmem (mk_rmem (post_f x `star` frame_f) h1) (post_f x)) /\
+      frame_opaque frame_f (focus_rmem m0 frame_f) (focus_rmem (mk_rmem (post_f x `star` frame_f) h1) frame_f))
+    ==> pr x /\
+      (can_be_split_trans (post_f x `star` frame_f) (pre_g x `star` frame_g x) (pre_g x);
+      (req_g x) (focus_rmem (mk_rmem (post_f x `star` frame_f) h1) (pre_g x))))
+
+unfold
+let bind_ens_opaque (#a:Type) (#b:Type)
+  (#pre_f:pre_t) (#post_f:post_t a)
+  (req_f:req_t pre_f) (ens_f:ens_t pre_f a post_f)
+  (#pre_g:a -> pre_t) (#post_g:a -> post_t b)
+  (#pr:a -> prop)
+  (ens_g:(x:a -> ens_t (pre_g x) b (post_g x)))
+  (frame_f:vprop) (frame_g:a -> vprop)
+  (post:post_t b)
+  (_:squash (can_be_split_forall_dep pr (fun x -> post_f x `star` frame_f) (fun x -> pre_g x `star` frame_g x)))
+  (_:squash (can_be_split_post (fun x y -> post_g x y `star` frame_g x) post))
+: ens_t (pre_f `star` frame_f) b post
+= fun m0 y m2 ->
+  req_f (focus_rmem m0 pre_f) /\
+  (exists (x:a) (h1:hmem (post_f x `star` frame_f)).
+    pr x /\
+    (
+    can_be_split_trans (post_f x `star` frame_f) (pre_g x `star` frame_g x) (pre_g x);
+    can_be_split_trans (post_f x `star` frame_f) (pre_g x `star` frame_g x) (frame_g x);
+    can_be_split_trans (post y) (post_g x y `star` frame_g x) (post_g x y);
+    can_be_split_trans (post y) (post_g x y `star` frame_g x) (frame_g x);
+    frame_opaque frame_f (focus_rmem m0 frame_f) (focus_rmem (mk_rmem (post_f x `star` frame_f) h1) frame_f) /\
+    frame_opaque (frame_g x) (focus_rmem (mk_rmem (post_f x `star` frame_f) h1) (frame_g x)) (focus_rmem m2 (frame_g x)) /\
+    ens_f (focus_rmem m0 pre_f) x (focus_rmem (mk_rmem (post_f x `star` frame_f) h1) (post_f x)) /\
+    (ens_g x) (focus_rmem (mk_rmem (post_f x `star` frame_f) h1) (pre_g x)) y (focus_rmem m2 (post_g x y))))
+
+val bind_opaque (a:Type) (b:Type)
+  (#framed_f:eqtype_as_type bool)
+  (#framed_g:eqtype_as_type bool)
+  (#pre_f:pre_t) (#post_f:post_t a)
+  (#req_f:req_t pre_f) (#ens_f:ens_t pre_f a post_f)
+  (#pre_g:a -> pre_t) (#post_g:a -> post_t b)
+  (#req_g:(x:a -> req_t (pre_g x))) (#ens_g:(x:a -> ens_t (pre_g x) b (post_g x)))
+  (#frame_f:vprop) (#frame_g:a -> vprop)
+  (#post:post_t b)
+  (# _ : squash (maybe_emp framed_f frame_f))
+  (# _ : squash (maybe_emp_dep framed_g frame_g))
+  (#pr:a -> prop)
+  (#p1:squash (can_be_split_forall_dep pr
+    (fun x -> post_f x `star` frame_f) (fun x -> pre_g x `star` frame_g x)))
+  (#p2:squash (can_be_split_post (fun x y -> post_g x y `star` frame_g x) post))
+  (f:repr a framed_f pre_f post_f req_f ens_f)
+  (g:(x:a -> repr b framed_g (pre_g x) (post_g x) (req_g x) (ens_g x)))
+: repr b
+    true
+    (pre_f `star` frame_f)
+    post
+    (bind_req_opaque req_f ens_f req_g frame_f frame_g p1)
+    (bind_ens_opaque req_f ens_f ens_g frame_f frame_g post p1 p2)
+
 
 #push-options "--z3rlimit 20"
-let bind a b #framed_f #framed_g #pre_f #post_f #req_f #ens_f #pre_g #post_g #req_g #ens_g #frame_f #frame_g #post #_ #_ #p #p2 f g =
+let bind_opaque a b #framed_f #framed_g #pre_f #post_f #req_f #ens_f #pre_g #post_g #req_g #ens_g #frame_f #frame_g #post #_ #_ #p #p2 f g =
   fun frame ->
     let m0 = nmst_get () in
 
@@ -296,6 +380,9 @@ let bind a b #framed_f #framed_g #pre_f #post_f #req_f #ens_f #pre_g #post_g #re
     y
 
 #pop-options
+
+let bind a b #framed_f #framed_g #pre_f #post_f #req_f #ens_f #pre_g #post_g #req_g #ens_g #frame_f #frame_g #post #_ #_ #p #p2 f g
+  = norm_repr (bind_opaque a b #framed_f #framed_g #pre_f #post_f #req_f #ens_f #pre_g #post_g #req_g #ens_g #frame_f #frame_g #post #_ #_ #p #p2 f g)
 
 /// Need to manually remove the rewrite_with_tactic marker here
 let lemma_unfold_subcomp_pre (#a:Type)
